formal/inference/Can_Take.thy
@@ -1,0 +1,182 @@
+theory Can_Take
+imports Inference
+begin
+
+unbundle finfun_syntax
+
+definition finfun2pairs :: "('a :: linorder) \<Rightarrow>f 'b \<Rightarrow> ('a \<times> 'b) list" where
+  "finfun2pairs f = (let keys = finfun_to_list f in zip keys (map (\<lambda>k. f $ k) keys))"
+
+fun null_guard :: "gexp \<Rightarrow> bool" where
+  "null_guard (Null _) = True" |
+  "null_guard (Nor g1 g2) = (null_guard g1 \<or> null_guard g2)" |
+  "null_guard _ = False"
+
+definition max_input :: "gexp list \<Rightarrow> nat option" where
+  "max_input g = (fold max (map (\<lambda>g. GExp.max_input g) g) None)"
+
+lemma max_input_cons: "Can_Take.max_input (a # G) = max (GExp.max_input a) (max_input G)"
+  apply (simp add: max_input_def)
+proof -
+  have "foldr max (GExp.max_input a # rev (map_tailrec GExp.max_input G)) None = foldr max (rev (None # map_tailrec GExp.max_input G)) (GExp.max_input a)"
+    by (metis (no_types) Max.set_eq_fold comp_def fold.simps(2) fold_conv_foldr foldr_conv_fold list.set(2) max.commute set_rev)
+  then show "fold max (map GExp.max_input G) (max (GExp.max_input a) None) = max (GExp.max_input a) (fold max (map GExp.max_input G) None)"
+    by (simp add: fold_conv_foldr map_eq_map_tailrec max.commute)
+qed
+
+lemma max_none: "max None x = x"
+  by (meson less_option.elims(2) linorder_not_le max.absorb2 option.distinct(1))
+
+lemma max_lt_val: "max (GExp.max_input a) (Can_Take.max_input G) = Some i \<Longrightarrow> (GExp.max_input a) \<le> Some i"
+  by (metis max.cobounded1)
+
+lemma Max_set_fold: "l \<noteq> [] \<Longrightarrow> Max (set (l)) = fold max l (hd l)"
+proof(induct l)
+  case Nil
+  then show ?case 
+    by simp
+next
+  case (Cons a l)
+  then show ?case
+    using Max.set_eq_fold by auto
+qed
+
+lemma max_union: "x \<noteq> [] \<Longrightarrow> y \<noteq> [] \<Longrightarrow> Max (set x \<union> set y) = max (Max (set x)) (Max (set y))"
+  by (simp add: Max.union)
+
+lemma in_not_empty: "x \<in> s \<Longrightarrow> s \<noteq> {}"
+  by auto
+
+lemma gexp_max_input_nor_aux: "x \<in> set (s1) \<Longrightarrow>
+       Some (Max (set (s1) \<union> set (s2))) \<noteq>
+       max (Some (Max (set (s1)))) (Some (Max (set (s2)))) \<Longrightarrow>
+       xa \<in> set (s2) \<Longrightarrow> False"
+  using in_not_empty[of x "set (s1)"]
+  using in_not_empty[of xa "set (s2)"]
+  apply simp
+  apply (simp add: max_union Max_set_fold)
+  by (metis less_option.simps(4) linorder_not_le max_def)
+
+lemma gexp_max_input_nor: "GExp.max_input (Nor g1 g2) = max (GExp.max_input g1) (GExp.max_input g2)"
+  apply (simp add: GExp.max_input_def Let_def)
+  apply safe
+    apply (simp add: max_none)
+   apply (simp add: max.commute max_none)
+  apply (simp add: enumerate_gexp_inputs_list)
+  using gexp_max_input_nor_aux by blast
+
+lemma max_input_Eq: "GExp.max_input (Eq a1 a2) = max (AExp.max_input a1) (AExp.max_input a2)"
+  apply (simp add: AExp.max_input_def GExp.max_input_def Let_def)
+  apply safe
+    apply (simp add: max_none)
+   apply (simp add: max.commute max_none)
+  apply simp
+  apply (simp add: enumerate_aexp_inputs_list enumerate_gexp_inputs_list)
+  using gexp_max_input_nor_aux by blast
+
+lemma max_input_Gt: "GExp.max_input (Gt a1 a2) = max (AExp.max_input a1) (AExp.max_input a2)"
+  apply (simp add: AExp.max_input_def GExp.max_input_def Let_def)
+  apply safe
+    apply (simp add: max_none)
+   apply (simp add: max.commute max_none)
+  apply simp
+  apply (simp add: enumerate_aexp_inputs_list enumerate_gexp_inputs_list)
+  by (metis gexp_max_input_nor_aux max.commute)
+
+lemma max_input_Plus: "AExp.max_input (Plus a1 a2) = max (AExp.max_input a1) (AExp.max_input a2)"
+  apply (simp add: AExp.max_input_def Let_def)
+  apply safe
+    apply (simp add: max_none)
+   apply (simp add: max.commute max_none)
+  apply simp
+  apply (simp add: enumerate_aexp_inputs_list enumerate_gexp_inputs_list)
+  using gexp_max_input_nor_aux by blast
+
+lemma max_input_Minus: "AExp.max_input (Minus a1 a2) = max (AExp.max_input a1) (AExp.max_input a2)"
+  apply (simp add: AExp.max_input_def Let_def)
+  apply safe
+    apply (simp add: max_none)
+   apply (simp add: max.commute max_none)
+  apply simp
+  apply (simp add: enumerate_aexp_inputs_list enumerate_gexp_inputs_list)
+  using gexp_max_input_nor_aux by blast
+
+lemma max_input_I: "AExp.max_input (V (vname.I i)) = Some i"
+  by (simp add: AExp.max_input_def)
+
+lemma "i < a \<Longrightarrow>
+    AExp.max_input x1a < Some i \<and> AExp.max_input x2 < Some i \<or> max (AExp.max_input x1a) (AExp.max_input x2) = Some i \<Longrightarrow>
+    aval x1a (join_ir ia r) = aval x2 (join_ir ia r) \<longrightarrow>
+    aval x1a (join_ir (take_or_pad ia a) r) = aval x2 (join_ir (take_or_pad ia a) r)"
+  apply (simp add: take_or_pad_def)
+  apply standard
+
+lemma "i < a \<Longrightarrow>
+    \<not> null_guard g \<Longrightarrow>
+    GExp.max_input g \<le> Some i \<Longrightarrow>
+    gval g (join_ir ia r) = gval g (join_ir (take_or_pad ia a) r)"
+proof(induct g)
+case (Bc x)
+  then show ?case
+    by (cases x, auto)
+next
+  case (Eq x1a x2)
+  then show ?case
+    apply simp
+    apply standard
+    apply (simp add: max_input_Eq)
+next
+  case (Gt x1a x2)
+  then show ?case sorry
+next
+  case (Nor g1 g2)
+  then show ?case 
+    apply (simp add: maybe_not_eq gexp_max_input_nor)
+    by (metis Nor.hyps(1) Nor.hyps(2) max.cobounded1 max.cobounded2)
+next
+  case (Null x)
+  then show ?case
+    by simp
+qed
+
+lemma 
+  "Can_Take.max_input G = Some i \<Longrightarrow>
+  i < a \<Longrightarrow>
+  \<forall>g\<in>set G. \<not> null_guard g \<Longrightarrow>
+  apply_guards G (join_ir ia r) \<Longrightarrow>
+  apply_guards G (join_ir (take_or_pad ia a) r)"
+proof(induct G)
+  case Nil
+  then show ?case
+    by simp
+next
+  case (Cons g G)
+  then show ?case
+    apply (simp add: apply_guards_cons max_input_cons)
+    using max_lt_val[of g G i]
+    apply simp
+qed
+
+lemma 
+  "max_input G = Some i \<Longrightarrow>
+  i < a \<Longrightarrow>
+  \<forall>g\<in>set G. \<not> null_guard g \<Longrightarrow>
+  \<exists>i r. gval (fold gAnd G (Bc True)) (join_ir i r) = true \<Longrightarrow>
+  \<exists>i. length i = a \<and> (\<exists>r. gval (fold gAnd G (Bc True)) (join_ir i r) = true)"
+    apply (simp only: fold_apply_guards apply_guards_cons)
+    apply clarify
+    apply (rule_tac x="take_or_pad ia a" in exI)
+    apply (simp add: length_take_or_pad)
+    apply (rule_tac x=r in exI)
+
+qed
+
+lemma 
+  "max_input (Guard t) = Some i \<Longrightarrow>
+   i < Arity t \<Longrightarrow>
+   \<forall>g \<in> set (Guard t). \<not> null_guard g \<Longrightarrow>
+   satisfiable_list (Guard t) \<Longrightarrow> \<exists>i r. can_take_transition t i r"
+  apply (simp add: can_take_transition_def satisfiable_list_def can_take_def satisfiable_def apply_guards_fold)
+
+
+end
